Propagate changes after constants renamings

specs/Spec.Chacha20Poly1305.fst
@@ -12,7 +12,7 @@ module Poly = Spec.Poly1305
 #set-options "--max_fuel 0 --z3rlimit 30"
 
 inline_for_extraction
-let size_key : size_nat =   32 (* in bytes *)
+let size_key : size_nat = 32 (* in bytes *)
 
 inline_for_extraction
 let size_nonce : size_nat = 12 (* in bytes *)
@@ -20,21 +20,21 @@ let size_nonce : size_nat = 12 (* in bytes *)
 type key = lbytes size_key
 type nonce = lbytes size_nonce
 
-let poly1305_padded (len:size_nat) (text:lbytes len) (tmp:lbytes Poly.blocksize) (st:Poly1305.state) : Poly1305.state =
-  let n = len / Poly.blocksize in
-  let r = len % Poly.blocksize in
-  let blocks = sub text 0 (n * Poly.blocksize) in
-  let rem = sub text (n * Poly.blocksize) r in
+let poly1305_padded (len:size_nat) (text:lbytes len) (tmp:lbytes Poly.size_block) (st:Poly1305.state) : Poly1305.state =
+  let n = len / Poly.size_block in
+  let r = len % Poly.size_block in
+  let blocks = sub text 0 (n * Poly.size_block) in
+  let rem = sub text (n * Poly.size_block) r in
   let st = Poly.update_blocks n blocks st in
   let tmp = update_sub tmp 0 r rem in
-  let st = Poly1305.update1 Poly1305.blocksize tmp st in
+  let st = Poly1305.update1 Poly1305.size_block tmp st in
   st
 
-let poly1305_do (k:Poly.key) (len:size_nat{len + Poly.blocksize <= max_size_t}) (m:lbytes len)
+let poly1305_do (k:Poly.key) (len:size_nat{len + Poly.size_block <= max_size_t}) (m:lbytes len)
         (aad_len:size_nat{(len + aad_len) / Spec.Chacha20.blocklen <= max_size_t}) (aad:lbytes aad_len)
 : Tot Poly.tag =
   let st = Poly.poly1305_init k in
-  let block = create Poly.blocksize (u8 0) in
+  let block = create Poly.size_block (u8 0) in
   let st = poly1305_padded aad_len aad block st in
   let st = poly1305_padded len m block st in
   let aad_len8 = uint_to_bytes_le #U64 (u64 aad_len) in
@@ -45,20 +45,20 @@ let poly1305_do (k:Poly.key) (len:size_nat{len + Poly.blocksize <= max_size_t}) 
   Poly.finish st
 
 
-val aead_encrypt: k:key -> n:nonce -> len:size_nat{len + Poly.blocksize <= max_size_t} -> m:lbytes len -> aad_len:size_nat{(len + aad_len) / Spec.Chacha20.blocklen <= max_size_t} -> aad:lbytes aad_len -> Tot (lbytes (len + Poly.blocksize))
+val aead_encrypt: k:key -> n:nonce -> len:size_nat{len + Poly.size_block <= max_size_t} -> m:lbytes len -> aad_len:size_nat{(len + aad_len) / Spec.Chacha20.blocklen <= max_size_t} -> aad:lbytes aad_len -> Tot (lbytes (len + Poly.size_block))
 
 let aead_encrypt k n len m len_aad aad =
   let key0 = Spec.Chacha20.chacha20_key_block0 k n in
   let poly_k = sub key0 0 32 in
-  let res = create (len + Poly.blocksize) (u8 0) in
+  let res = create (len + Poly.size_block) (u8 0) in
   let cipher = Spec.Chacha20.chacha20_encrypt_bytes k n 1 len m in
   let mac = poly1305_do poly_k len cipher len_aad aad in
   let res = update_sub res 0 len cipher in
-  let res = update_sub res len Poly.blocksize mac in
+  let res = update_sub res len Poly.size_block mac in
   res
 
 
-val aead_decrypt: k:key -> n:nonce -> len:size_nat{len + Poly.blocksize <= max_size_t} -> c:lbytes len -> tag:lbytes Poly.blocksize -> aad_len:size_nat{(len + aad_len) / Spec.Chacha20.blocklen <= max_size_t} -> aad:lbytes aad_len -> Tot (option (lbytes len))
+val aead_decrypt: k:key -> n:nonce -> len:size_nat{len + Poly.size_block <= max_size_t} -> c:lbytes len -> tag:lbytes Poly.size_block -> aad_len:size_nat{(len + aad_len) / Spec.Chacha20.blocklen <= max_size_t} -> aad:lbytes aad_len -> Tot (option (lbytes len))
 let aead_decrypt k n len c tag len_aad aad =
   let key0 = Spec.Chacha20.chacha20_key_block0 k n in
   let poly_k = sub key0 0 32 in
